tests/mutual.v
@@ -1,3 +1,5 @@
+From HB Require Import structures.
+
 From mathcomp Require Import
   ssreflect ssrfun ssrbool ssrnat eqtype seq choice fintype finset order.
 
@@ -32,35 +34,26 @@ Canonical bar_indType := IndType bar foo_bar_baz_indDef.
 Canonical baz_indType := IndType baz foo_bar_baz_indDef.
 
 Definition foo_eqMixin := [derive lazy eqMixin for foo].
-Canonical foo_eqType := EqType foo foo_eqMixin.
+HB.instance Definition _ := foo_eqMixin.
 Definition bar_eqMixin := [derive lazy eqMixin for bar].
-Canonical bar_eqType := EqType bar bar_eqMixin.
+HB.instance Definition _ := bar_eqMixin.
 Definition baz_eqMixin := [derive lazy eqMixin for baz].
-Canonical baz_eqType := EqType baz baz_eqMixin.
+HB.instance Definition _ := baz_eqMixin.
 Definition foo_choiceMixin := [derive choiceMixin for foo].
-Canonical foo_choiceType := Eval hnf in ChoiceType foo foo_choiceMixin.
+HB.instance Definition _ := foo_choiceMixin.
 Definition bar_choiceMixin := [derive choiceMixin for bar].
-Canonical bar_choiceType := Eval hnf in ChoiceType bar bar_choiceMixin.
+HB.instance Definition _ := bar_choiceMixin.
 Definition baz_choiceMixin := [derive choiceMixin for baz].
-Canonical baz_choiceType := Eval hnf in ChoiceType baz baz_choiceMixin.
+HB.instance Definition _ := baz_choiceMixin.
 Definition foo_countMixin := [derive countMixin for foo].
-Canonical foo_countType := Eval hnf in CountType foo foo_countMixin.
+HB.instance Definition _ := foo_countMixin.
 Definition bar_countMixin := [derive countMixin for bar].
-Canonical bar_countType := Eval hnf in CountType bar bar_countMixin.
+HB.instance Definition _ := bar_countMixin.
 Definition baz_countMixin := [derive countMixin for baz].
-Canonical baz_countType := Eval hnf in CountType baz baz_countMixin.
+HB.instance Definition _ := baz_countMixin.
 Definition foo_orderMixin := [derive lazy orderMixin for foo].
-Canonical foo_porderType := Eval hnf in POrderType tt foo foo_orderMixin.
-Canonical foo_latticeType := Eval hnf in LatticeType foo foo_orderMixin.
-Canonical foo_distrLatticeType := Eval hnf in DistrLatticeType foo foo_orderMixin.
-Canonical foo_orderType := Eval hnf in OrderType foo foo_orderMixin.
+HB.instance Definition _ := foo_orderMixin.
 Definition bar_orderMixin := [derive lazy orderMixin for bar].
-Canonical bar_porderType := Eval hnf in POrderType tt bar bar_orderMixin.
-Canonical bar_latticeType := Eval hnf in LatticeType bar bar_orderMixin.
-Canonical bar_distrLatticeType := Eval hnf in DistrLatticeType bar bar_orderMixin.
-Canonical bar_orderType := Eval hnf in OrderType bar bar_orderMixin.
+HB.instance Definition _ := bar_orderMixin.
 Definition baz_orderMixin := [derive lazy orderMixin for baz].
-Canonical baz_porderType := Eval hnf in POrderType tt baz baz_orderMixin.
-Canonical baz_latticeType := Eval hnf in LatticeType baz baz_orderMixin.
-Canonical baz_distrLatticeType := Eval hnf in DistrLatticeType baz baz_orderMixin.
-Canonical baz_orderType := Eval hnf in OrderType baz baz_orderMixin.
+HB.instance Definition _ := baz_orderMixin.
