tests/records.v
@@ -1,3 +1,4 @@
+From HB Require Import structures.
 From mathcomp Require Import all_ssreflect.
 From deriving Require Import deriving.
 
@@ -7,8 +8,8 @@ Scheme foo_rect := Induction for foo Sort Type.
 Definition foo_indDef := [indDef for foo_rect].
 Canonical foo_indType := IndType foo foo_indDef.
 Definition foo_eqMixin := [derive eqMixin for foo].
-Canonical foo_eqType := EqType foo foo_eqMixin.
+HB.instance Definition _ := foo_eqMixin.
 Definition foo_choiceMixin := [derive choiceMixin for foo].
-Canonical foo_choiceType := Eval hnf in ChoiceType foo foo_choiceMixin.
+HB.instance Definition _ := foo_choiceMixin.
 Definition foo_countMixin := [derive countMixin for foo].
-Canonical foo_countType := Eval hnf in CountType foo foo_countMixin.
+HB.instance Definition _ := foo_countMixin.
