tests/three.v
@@ -1,3 +1,5 @@
+From HB Require Import structures.
+
 From mathcomp Require Import
   ssreflect ssrfun ssrbool ssrnat eqtype seq choice fintype finset order.
 
@@ -16,27 +18,16 @@ Canonical three_indType :=
 
 Definition three_eqMixin :=
   [derive eqMixin for three].
-Canonical three_eqType :=
-  Eval hnf in EqType three three_eqMixin.
+HB.instance Definition _ := three_eqMixin.
 Definition three_choiceMixin :=
   [derive choiceMixin for three].
-Canonical three_choiceType :=
-  Eval hnf in ChoiceType three three_choiceMixin.
+HB.instance Definition _ := three_choiceMixin.
 Definition three_countMixin :=
   [derive countMixin for three].
-Canonical three_countType :=
-  Eval hnf in CountType three three_countMixin.
+HB.instance Definition _ := three_countMixin.
 Definition three_finMixin :=
   [derive finMixin for three].
-Canonical three_finType :=
-  Eval hnf in FinType three three_finMixin.
+HB.instance Definition _ := three_finMixin.
 Definition three_orderMixin :=
   [derive lazy orderMixin for three].
-Canonical three_porderType :=
-  Eval hnf in POrderType tt three three_orderMixin.
-Canonical three_latticeType :=
-  Eval hnf in LatticeType three three_orderMixin.
-Canonical three_distrLatticeType :=
-  Eval hnf in DistrLatticeType three three_orderMixin.
-Canonical three_orderType :=
-  Eval hnf in OrderType three three_orderMixin.
+HB.instance Definition _ := three_orderMixin.
